[llir-semantics] Progress on SSA validity.

Verify.v
@@ -32,7 +32,11 @@ Section VALIDITY.
     forall (def: node) (use: node),
       StrictlyDominates f def use -> Pos.lt def use.
 
-  Definition is_valid := uses_have_defs /\ defs_are_unique /\ well_ordered.
+  Record is_valid : Prop :=
+    { fn_uses_have_defs: uses_have_defs
+    ; fn_defs_are_unique: defs_are_unique
+    ; fn_well_ordered: well_ordered
+    }.
 
   Theorem defs_dominate_uses:
     is_valid ->
@@ -42,7 +46,7 @@ Section VALIDITY.
       StrictlyDominates f def use.
   Proof.
     intros Hvalid def use r.
-    destruct Hvalid as [Huses_have_defs [Hdefs_are_unique _]].
+    destruct Hvalid as [Huses_have_defs Hdefs_are_unique _].
     intros Hdef.
     intros Huse.
     unfold uses_have_defs in Huses_have_defs.
@@ -51,5 +55,29 @@ Section VALIDITY.
     destruct Hdom as [dom [Hdef' Hdom]].
     generalize (Hdefs_are_unique def dom r Hdef Hdef').
     intros Heq. subst. auto.
+  Qed.
+
+  Theorem no_use_of_def:
+    is_valid ->
+    forall (n: node) (r: reg),
+      DefinedAt f n r -> ~ (UsedAt f n r).
+  Proof.
+    intros Hvalid n r Hdef Huse.
+    generalize (defs_dominate_uses Hvalid n n r Hdef Huse).
+    intros Hdom.
+    inversion Hdom.
+    auto.
+  Qed.
+
+  Theorem no_def_of_use:
+    is_valid ->
+    forall (n: node) (r: reg),
+      UsedAt f n r -> ~ (DefinedAt f n r).
+  Proof.
+    intros Hvalid n r Huse Hdef.
+    generalize(defs_dominate_uses Hvalid n n r Hdef Huse).
+    intros Hdom.
+    inversion Hdom.
+    auto.
   Qed.
 End VALIDITY.
